projection/proofs/ffi/comms_ffi_commScript.sml
@@ -1,0 +1,602 @@
+open HolKernel boolLib Parse bossLib;
+open optionTheory
+     relationTheory;
+open ffiTheory;
+open bisimulationTheory
+     confluenceTheory
+     payloadPropsTheory
+     payloadSemanticsTheory
+     payloadLangTheory
+     comms_ffi_modelTheory
+     comms_ffi_propsTheory
+     comms_ffi_consTheory;
+
+val _ = new_theory "comms_ffi_comm";
+
+(* INTER-PIECE COMMUTATIVITY *)
+(* Internal Commutativity *)
+(* -- internal/active *)
+Theorem internal_active_comm:
+  ∀conf c S1 S2A S2B.
+    ffi_wf (c,S1) ∧
+    RTC (internal_trans conf c) S1 S2A ∧
+    RTC (active_trans conf c) S1 S2B ⇒
+    ∃S3.
+      RTC (active_trans conf c) S2A S3 ∧
+      RTC (internal_trans conf c) S2B S3
+Proof
+  rw[] >>
+  irule rc_diam_to_rtc_diam >> 
+  MAP_EVERY qexists_tac [‘S1’,‘(λx. ffi_wf (c,x))’] >>
+  rw[]
+  >- (rename [‘_ _ _ S1f S2Af’,‘_ _ _ S1f S2Bf’,
+              ‘RC _ S2Af _ ∧ RC _ S2Bf _’] >>
+      rpt (qpat_x_assum ‘RTC _ _ _’ (K ALL_TAC)) >>
+      MAP_EVERY PairCases_on [‘S1f’,‘S2Af’,‘S2Bf’] >>
+      ‘∀ i j k l.
+        RC (internal_trans conf c) (i,j) (k,l) =
+          (i = k ∧ RC (λn1 n2. trans conf n1 LTau n2) j l)’
+        by (fs[RC_DEF,internal_trans_def] >> metis_tac[]) >>
+      ‘∀ i j k l.
+        RC (emit_trans conf c) (i,j) (k,l) =
+          ((i = k ∧ j = l) ∨
+           (∃sp d.
+              k = qpush i sp d ∧
+              (λn1 n2. trans conf n1 (LSend sp d c) n2) j l))’
+        by (fs[RC_DEF,emit_trans_def] >> metis_tac[]) >>
+      fs[active_trans_def]
+      >- (‘∃S3.
+            RC (internal_trans conf c) (S2Af0,S2Af1) S3 ∧
+            RC (internal_trans conf c) (S2Bf0,S2Bf1) S3’
+            suffices_by (rw[] >> qexists_tac ‘S3’ >>
+                         pop_assum (assume_tac o
+                                    REWRITE_RULE [RC_DEF]) >>
+                         PairCases_on ‘S3’ >>
+                         fs[RC_DEF,active_trans_def]) >>
+          fs[internal_trans_def,pairTheory.EXISTS_PROD] >>
+          irule trans_diamond >> rw[compat_labels_def] >>
+          qexists_tac ‘S1f1’ >> fs[wf_label_def,ffi_wf_def])
+      >- (‘∃S3.
+            RC (emit_trans conf c) (S2Af0,S2Af1) S3 ∧
+            RC (internal_trans conf c) (S2Bf0,S2Bf1) S3’
+            suffices_by (rw[] >> qexists_tac ‘S3’ >>
+                         pop_assum (assume_tac o
+                                    REWRITE_RULE [RC_DEF]) >>
+                         PairCases_on ‘S3’ >>
+                         fs[RC_DEF,active_trans_def]) >>
+          fs[internal_trans_def,emit_trans_def,pairTheory.EXISTS_PROD] >>
+          qspecl_then [‘S1f1’,‘LTau’,‘S2Af1’,
+                       ‘LSend sp d c’,‘S2Bf1’]
+                      assume_tac trans_diff_diamond >>
+          rfs[ffi_wf_def,compat_labels_def,wf_label_def] >>
+          rename [‘trans conf S2Bf1 LTau N3’,
+                  ‘trans conf S2Af1 (LSend sp d c) N3’] >>
+          qexists_tac ‘N3’ >> rw[RC_DEF] >>
+          metis_tac[]))
+  >- (rename [‘ffi_wf (c,ks)’,‘internal_trans conf c ks us’] >>
+      MAP_EVERY PairCases_on [‘ks’,‘us’] >>
+      metis_tac[trans_pres_wf,trans_pres_nodes,
+                ffi_wf_def,internal_trans_def])
+  >- (rename [‘ffi_wf (c,ks)’,‘active_trans conf c ks us’] >>
+      MAP_EVERY PairCases_on [‘ks’,‘us’] >>
+      metis_tac[trans_pres_wf,trans_pres_nodes,
+                ffi_wf_def,active_trans_def,
+                internal_trans_def,emit_trans_def])
+QED
+
+(* -- internal/send *)
+Theorem internal_send_comm:
+  ∀conf c S1 S2A S2B ML.
+    ffi_wf (c,S1) ∧
+    RTC (internal_trans conf c) S1 S2A ∧
+    input_trans conf c S1 ML S2B ⇒
+    ∃S3.
+      input_trans conf c S2A ML S3 ∧
+      RTC (internal_trans conf c) S2B S3
+Proof
+  rw[] >>
+  qspecl_then [‘internal_trans conf c’,
+               ‘(λn1 n2. input_trans conf c n1 ML n2)’,
+               ‘(λx. ffi_wf (c,x))’]
+              assume_tac
+              diam_to_srtc_diam >> 
+  qmatch_asmsub_abbrev_tac ‘A ⇒ B’ >>
+  ‘A’
+    suffices_by (rw[] >> fs[] >>
+                 qunabbrev_tac ‘B’ >>
+                 pop_assum (K ALL_TAC) >>
+                 first_x_assum irule >>
+                 metis_tac[]) >>
+  ntac 4 (last_x_assum (K ALL_TAC)) >>
+  MAP_EVERY qunabbrev_tac [‘A’,‘B’] >>
+  rw[]
+  >- (rename [‘ffi_wf (c,ks)’,‘internal_trans conf c ks us’] >>
+      MAP_EVERY PairCases_on [‘ks’,‘us’] >>
+      metis_tac[trans_pres_wf,trans_pres_nodes,
+                ffi_wf_def,internal_trans_def])
+  >- (rename [‘ffi_wf (c,ks)’,‘input_trans conf c ks ML us’] >>
+      MAP_EVERY PairCases_on [‘ks’,‘ML’,‘us’] >>
+      metis_tac[trans_pres_wf,trans_pres_nodes,
+                ffi_wf_def,input_trans_def])
+  >- (MAP_EVERY PairCases_on [‘S1’,‘S2A’,‘ML’,‘S2B’] >>
+      fs[input_trans_def,internal_trans_def,
+         pairTheory.EXISTS_PROD] >>
+      irule trans_diff_diamond >>
+      fs[ffi_wf_def,compat_labels_def,wf_label_def] >>
+      metis_tac[])
+QED
+
+(* -- internal/receive *)
+Theorem internal_rec_comm:
+  ∀conf c S1 S2A S2B ML.
+    ffi_wf (c,S1) ∧
+    RTC (internal_trans conf c) S1 S2A ∧
+    output_trans conf c S1 ML S2B ⇒
+    ∃S3.
+      output_trans conf c S2A ML S3 ∧
+      RTC (internal_trans conf c) S2B S3
+Proof
+  rw[pairTheory.EXISTS_PROD] >>
+  MAP_EVERY PairCases_on [‘S1’,‘S2A’,‘S2B’,‘ML’] >>
+  ‘S2A0 = S10’
+    by (qpat_x_assum ‘RTC _ _ _’ mp_tac >>
+        MAP_EVERY qid_spec_tac [‘S10’,‘S11’,‘S2A0’,‘S2A1’] >>
+        Induct_on ‘RTC’ >> rw[] >> rename1 ‘RTC _ SI _’ >>
+        PairCases_on ‘SI’ >> fs[internal_trans_def]) >>
+  ‘S2B1 = S11’
+    by fs[output_trans_def] >>
+  fs[] >>
+  MAP_EVERY qexists_tac [‘S2B0’,‘S2A1’] >>
+  rw[] >- fs[output_trans_def] >>
+  last_x_assum (K ALL_TAC) >>
+  pop_assum (K ALL_TAC) >>
+  pop_assum mp_tac >>
+  MAP_EVERY qid_spec_tac [‘S10’,‘S11’,‘S2B0’,‘S2A1’] >>
+  Induct_on ‘RTC’ >> rw[]
+  >- metis_tac[RTC_REFL] >>
+  rename1 ‘RTC _ SI (S10,S2A1)’ >>
+  PairCases_on ‘SI’ >>
+  ‘S10 = SI0’
+    by fs[internal_trans_def] >>
+  fs[] >> 
+  ‘internal_trans conf c (S2B0,S11) (S2B0,SI1)’
+    suffices_by metis_tac[RTC_TRANSITIVE,transitive_def,RTC_SINGLE] >>
+  fs[internal_trans_def]
+QED
+
+(* -- internal/internal *)
+Theorem internal_internal_comm:
+  ∀conf c S1 S2A S2B.
+    ffi_wf (c,S1) ∧
+    RTC (internal_trans conf c) S1 S2A ∧
+    RTC (internal_trans conf c) S1 S2B ⇒
+    ∃S3.
+      RTC (internal_trans conf c) S2A S3 ∧
+      RTC (internal_trans conf c) S2B S3
+Proof
+  rw[] >>
+  irule rc_diam_to_rtc_diam >> 
+  MAP_EVERY qexists_tac [‘S1’,‘(λx. ffi_wf (c,x))’] >>
+  rw[]
+  >- (rename [‘_ _ _ S1f S2Af’,‘_ _ _ S1f S2Bf’,
+              ‘RC _ S2Af _ ∧ RC _ S2Bf _’] >>
+      rpt (qpat_x_assum ‘RTC _ _ _’ (K ALL_TAC)) >>
+      MAP_EVERY PairCases_on [‘S1f’,‘S2Af’,‘S2Bf’] >>
+      ‘∀ i j k l.
+        RC (internal_trans conf c) (i,j) (k,l) =
+          (i = k ∧ RC (λn1 n2. trans conf n1 LTau n2) j l)’
+        by (fs[RC_DEF,internal_trans_def] >> metis_tac[]) >>
+      fs[internal_trans_def,pairTheory.EXISTS_PROD] >>
+      irule trans_diamond >> rw[compat_labels_def] >>
+      qexists_tac ‘S1f1’ >>
+      fs[wf_label_def,ffi_wf_def])
+  >- (rename [‘ffi_wf (c,ks)’,‘internal_trans conf c ks us’] >>
+      MAP_EVERY PairCases_on [‘ks’,‘us’] >>
+      metis_tac[trans_pres_wf,trans_pres_nodes,
+                ffi_wf_def,internal_trans_def])
+  >- (rename [‘ffi_wf (c,ks)’,‘internal_trans conf c ks us’] >>
+      MAP_EVERY PairCases_on [‘ks’,‘us’] >>
+      metis_tac[trans_pres_wf,trans_pres_nodes,
+                ffi_wf_def,internal_trans_def])
+QED
+
+(* Active Commutativity *)
+(* -- active/active *)
+Theorem active_active_comm:
+  ∀conf c S1 S2A S2B.
+    ffi_wf (c,S1) ∧
+    RTC (active_trans conf c) S1 S2A ∧
+    RTC (active_trans conf c) S1 S2B ⇒
+    ∃S3.
+      RTC (active_trans conf c) S2A S3 ∧
+      RTC (active_trans conf c) S2B S3
+Proof
+  rw[] >>
+  irule rc_diam_to_rtc_diam >> 
+  MAP_EVERY qexists_tac [‘S1’,‘(λx. ffi_wf (c,x))’] >>
+  rw[]
+  >- (rename [‘_ _ _ S1f S2Af’,‘_ _ _ S1f S2Bf’,
+              ‘RC _ S2Af _ ∧ RC _ S2Bf _’] >>
+      rpt (qpat_x_assum ‘RTC _ _ _’ (K ALL_TAC)) >>
+      MAP_EVERY PairCases_on [‘S1f’,‘S2Af’,‘S2Bf’] >>
+      ‘∀ i j k l.
+        RC (internal_trans conf c) (i,j) (k,l) =
+          (i = k ∧ RC (λn1 n2. trans conf n1 LTau n2) j l)’
+        by (fs[RC_DEF,internal_trans_def] >> metis_tac[]) >>
+      ‘∀ i j k l.
+        RC (emit_trans conf c) (i,j) (k,l) =
+          ((i = k ∧ j = l) ∨
+           (∃sp d.
+              k = qpush i sp d ∧
+              (λn1 n2. trans conf n1 (LSend sp d c) n2) j l))’
+        by (fs[RC_DEF,emit_trans_def] >> metis_tac[]) >>
+      fs[active_trans_def]
+      >- (‘∃S3.
+            RC (internal_trans conf c) (S2Af0,S2Af1) S3 ∧
+            RC (internal_trans conf c) (S2Bf0,S2Bf1) S3’
+            suffices_by (rw[] >> qexists_tac ‘S3’ >>
+                         pop_assum (assume_tac o
+                                    REWRITE_RULE [RC_DEF]) >>
+                         PairCases_on ‘S3’ >>
+                         fs[RC_DEF,active_trans_def]) >>
+          fs[internal_trans_def,pairTheory.EXISTS_PROD] >>
+          irule trans_diamond >> rw[compat_labels_def] >>
+          qexists_tac ‘S1f1’ >> fs[wf_label_def,ffi_wf_def])
+      >- (‘∃S3.
+            RC (emit_trans conf c) (S2Af0,S2Af1) S3 ∧
+            RC (internal_trans conf c) (S2Bf0,S2Bf1) S3’
+            suffices_by (rw[] >> qexists_tac ‘S3’ >>
+                         pop_assum (assume_tac o
+                                    REWRITE_RULE [RC_DEF]) >>
+                         PairCases_on ‘S3’ >>
+                         fs[RC_DEF,active_trans_def]) >>
+          fs[internal_trans_def,emit_trans_def,pairTheory.EXISTS_PROD] >>
+          qspecl_then [‘S1f1’,‘LTau’,‘S2Af1’,
+                       ‘LSend sp d c’,‘S2Bf1’]
+                      assume_tac trans_diff_diamond >>
+          rfs[ffi_wf_def,compat_labels_def,wf_label_def] >>
+          rename [‘trans conf S2Bf1 LTau N3’,
+                  ‘trans conf S2Af1 (LSend sp d c) N3’] >>
+          qexists_tac ‘N3’ >> rw[RC_DEF] >>
+          metis_tac[])
+    >- (‘∃S3.
+          RC (internal_trans conf c) (S2Af0,S2Af1) S3 ∧
+          RC (emit_trans conf c) (S2Bf0,S2Bf1) S3’
+          suffices_by (rw[] >> qexists_tac ‘S3’ >>
+                       pop_assum (assume_tac o
+                                  REWRITE_RULE [RC_DEF]) >>
+                       PairCases_on ‘S3’ >>
+                       fs[RC_DEF,active_trans_def]) >>
+        fs[internal_trans_def,emit_trans_def,pairTheory.EXISTS_PROD] >>
+        qspecl_then [‘S1f1’,‘LSend sp d c’,‘S2Af1’,
+                     ‘LTau’,‘S2Bf1’]
+                    assume_tac trans_diff_diamond >>
+        rfs[ffi_wf_def,compat_labels_def,wf_label_def] >>
+        rename [‘trans conf S2Bf1 (LSend sp d c) N3’,
+                ‘trans conf S2Af1 LTau N3’] >>
+        qexists_tac ‘N3’ >> rw[RC_DEF] >>
+        metis_tac[])
+    >- (‘∃S3.
+          RC (emit_trans conf c) (S2Af0,S2Af1) S3 ∧
+          RC (emit_trans conf c) (S2Bf0,S2Bf1) S3’
+          suffices_by (rw[] >> qexists_tac ‘S3’ >>
+                       pop_assum (assume_tac o
+                                  REWRITE_RULE [RC_DEF]) >>
+                       PairCases_on ‘S3’ >>
+                       fs[RC_DEF,active_trans_def]) >>
+        fs[emit_trans_def,pairTheory.EXISTS_PROD] >>
+        rename1 ‘trans conf S1f1 (LSend spA dA c) S2Af1’ >>
+        rename1 ‘trans conf S1f1 (LSend spB dB c) S2Bf1’ >>
+        Cases_on ‘spA = spB’
+        >- (‘dA = dB’
+              by (‘compat_labels (LReceive spA dA c) (LReceive spB dB c)’
+                    suffices_by rw[compat_labels_def] >>
+                  metis_tac[ffi_wf_def,send_gen_compat]) >>
+            fs[] >>
+            ‘S2Af1 = S2Bf1’
+              by (irule trans_notau_functional >>
+                  MAP_EVERY qexists_tac [‘LSend spB dB c’,‘S1f1’,‘conf’] >>
+                  fs[ffi_wf_def]) >>
+            MAP_EVERY qexists_tac [‘qpush S1f0 spB dB’,‘S2Af1’] >>
+            rw[])
+        >- (qspecl_then [‘S1f1’,‘LSend spA dA c’,‘S2Af1’,
+                         ‘LSend spB dB c’,‘S2Bf1’]
+                        assume_tac trans_diff_diamond >>
+            rfs[ffi_wf_def,compat_labels_def,wf_label_def] >>
+            rename [‘trans conf S2Bf1 (LSend spA dA c) N3’,
+                    ‘trans conf S2Af1 (LSend spB dB c) N3’] >>
+            MAP_EVERY qexists_tac
+                      [‘qpush (qpush S1f0 spA dA) spB dB’,
+                       ‘N3’] >> rw[] >>
+            metis_tac[qpush_commutes])))
+  >- (rename [‘ffi_wf (c,ks)’,‘active_trans conf c ks us’] >>
+      MAP_EVERY PairCases_on [‘ks’,‘us’] >>
+      metis_tac[trans_pres_wf,trans_pres_nodes,
+                ffi_wf_def,active_trans_def,
+                internal_trans_def,emit_trans_def])
+  >- (rename [‘ffi_wf (c,ks)’,‘active_trans conf c ks us’] >>
+      MAP_EVERY PairCases_on [‘ks’,‘us’] >>
+      metis_tac[trans_pres_wf,trans_pres_nodes,
+                ffi_wf_def,active_trans_def,
+                internal_trans_def,emit_trans_def])
+QED
+(* -- active/send *)
+Theorem active_send_comm:
+  ∀conf c S1 S2A S2B ML.
+    ffi_wf (c,S1) ∧
+    RTC (active_trans conf c) S1 S2A ∧
+    input_trans conf c S1 ML S2B ⇒
+    ∃S3.
+      input_trans conf c S2A ML S3 ∧
+      RTC (active_trans conf c) S2B S3
+Proof
+  rw[] >>
+  qspecl_then [‘active_trans conf c’,
+               ‘(λn1 n2. input_trans conf c n1 ML n2)’,
+               ‘(λx. ffi_wf (c,x))’]
+              assume_tac
+              diam_to_srtc_diam >> 
+  qmatch_asmsub_abbrev_tac ‘A ⇒ B’ >>
+  ‘A’
+    suffices_by (rw[] >> fs[] >>
+                 qunabbrev_tac ‘B’ >>
+                 pop_assum (K ALL_TAC) >>
+                 first_x_assum irule >>
+                 metis_tac[]) >>
+  ntac 4 (last_x_assum (K ALL_TAC)) >>
+  MAP_EVERY qunabbrev_tac [‘A’,‘B’] >>
+  rw[]
+  >- (rename [‘ffi_wf (c,ks)’,‘active_trans conf c ks us’] >>
+      MAP_EVERY PairCases_on [‘ks’,‘us’] >>
+      metis_tac[trans_pres_wf,trans_pres_nodes,
+                ffi_wf_def,active_trans_def,
+                internal_trans_def,emit_trans_def])
+  >- (rename [‘ffi_wf (c,ks)’,‘input_trans conf c ks ML us’] >>
+      MAP_EVERY PairCases_on [‘ks’,‘ML’,‘us’] >>
+      metis_tac[trans_pres_wf,trans_pres_nodes,
+                ffi_wf_def,input_trans_def])
+  >- (MAP_EVERY PairCases_on [‘S1’,‘S2A’,‘ML’,‘S2B’] >>
+      fs[pairTheory.EXISTS_PROD,active_trans_def]
+      >- (‘∃N30 N31.
+            input_trans conf c (S2A0,S2A1) (ML0,ML1) (N30,N31) ∧
+            internal_trans conf c (S2B0,S2B1) (N30,N31)’
+            suffices_by metis_tac[] >>
+          fs[input_trans_def,internal_trans_def] >>
+          irule trans_diff_diamond >>
+          fs[ffi_wf_def,compat_labels_def,wf_label_def] >>
+          metis_tac[])
+      >- (‘∃N30 N31.
+            input_trans conf c (S2A0,S2A1) (ML0,ML1) (N30,N31) ∧
+            emit_trans conf c (S2B0,S2B1) (N30,N31)’
+            suffices_by metis_tac[] >>
+          fs[input_trans_def,emit_trans_def] >>
+          rename1 ‘trans conf S11 (LSend sp dA c) S2A1’ >>
+          rename1 ‘trans conf S11 (LReceive c dB rp) S2B1’ >>
+          qspecl_then [‘S11’,‘LSend sp dA c’,‘S2A1’,
+                       ‘LReceive c dB rp’,‘S2B1’]
+                      assume_tac trans_diff_diamond >>
+          rfs[ffi_wf_def,wf_label_def,compat_labels_def] >>
+          qexists_tac ‘N3’ >> rw[] >> metis_tac[]))
+QED
+
+(* -- active/receive *)
+Theorem active_rec_comm:
+  ∀conf c S1 S2A S2B ML.
+    ffi_wf (c,S1) ∧
+    RTC (active_trans conf c) S1 S2A ∧
+    output_trans conf c S1 ML S2B ⇒
+    ∃S3.
+      output_trans conf c S2A ML S3 ∧
+      RTC (active_trans conf c) S2B S3
+Proof
+  rw[pairTheory.EXISTS_PROD] >>
+  MAP_EVERY PairCases_on [‘S1’,‘S2A’,‘S2B’,‘ML’] >>
+  ‘S2B1 = S11’
+    by fs[output_trans_def] >>
+  fs[] >>
+  pop_assum (K ALL_TAC) >>
+  ntac 2 (pop_assum mp_tac) >>
+  pop_assum (K ALL_TAC) >>
+  MAP_EVERY qid_spec_tac [‘S10’,‘S11’,‘S2B0’,‘S2A1’] >>
+  Induct_on ‘RTC’ >> rw[]
+  >- metis_tac[RTC_REFL] >>
+  rename1 ‘RTC _ SI (S2A0,S2A1)’ >>
+  PairCases_on ‘SI’ >>
+  pop_assum (qspecl_then [‘SI1’,‘SI0’] assume_tac) >>
+  fs[] >>
+  ‘∃SG0 SG1.
+    output_trans conf c (SI0,SI1) (ML0,ML1) (SG0,SG1) ∧
+    active_trans conf c (S2B0,S11) (SG0,SG1)’
+    suffices_by (rw[] >>
+                 ‘SG1 = SI1’
+                   by fs[output_trans_def] >>
+                 fs[] >> last_x_assum (drule_all_then strip_assume_tac) >>
+                 metis_tac[RTC_TRANSITIVE,transitive_def,RTC_SINGLE]) >>
+  pop_assum (K ALL_TAC) >>
+  qpat_x_assum ‘RTC _ _ _’ (K ALL_TAC) >>
+  last_x_assum (assume_tac o REWRITE_RULE [active_trans_def]) >>
+  fs[]
+  >- (‘∃SG0 SG1.
+        output_trans conf c (SI0,SI1) (ML0,ML1) (SG0,SG1) ∧
+        internal_trans conf c (S2B0,S11) (SG0,SG1)’
+        suffices_by metis_tac[active_trans_def] >>
+      fs[output_trans_def,internal_trans_def])
+  >- (‘∃SG0 SG1.
+        output_trans conf c (SI0,SI1) (ML0,ML1) (SG0,SG1) ∧
+        emit_trans conf c (S2B0,S11) (SG0,SG1)’
+        suffices_by metis_tac[active_trans_def] >>
+      fs[output_trans_def,emit_trans_def] >>
+      qexists_tac ‘qpush S2B0 sp d’ >> rw[]
+      >- (rw[qpush_def] >>
+          Cases_on ‘ML0 = sp’
+          >- (rw[qlk_def,fget_def] >>
+              Cases_on ‘FLOOKUP S2B0 ML0’ >>
+              simp[finite_mapTheory.FLOOKUP_UPDATE])
+          >- (rw[qlk_def,fget_def] >> 
+              MAP_EVERY Cases_on [‘FLOOKUP S2B0 ML0’,‘FLOOKUP S2B0 sp’] >>
+              simp[finite_mapTheory.FLOOKUP_UPDATE,
+                   finite_mapTheory.FUPDATE_COMMUTES]))
+      >- (rw[qpush_def] >>
+          Cases_on ‘ML0 = sp’
+          >- (rw[qlk_def,fget_def] >>
+              Cases_on ‘FLOOKUP S2B0 ML0’ >>
+              simp[finite_mapTheory.FLOOKUP_UPDATE])
+          >- (fs[qlk_def,fget_def] >> 
+              MAP_EVERY Cases_on [‘FLOOKUP S2B0 ML0’,‘FLOOKUP S2B0 sp’] >>
+              fs[finite_mapTheory.FLOOKUP_UPDATE,
+                 finite_mapTheory.FUPDATE_COMMUTES] >>
+              metis_tac[]))
+      >- metis_tac[])
+QED
+
+(* -- active/internal *)
+Theorem active_internal_comm:
+  ∀conf c S1 S2A S2B.
+    ffi_wf (c,S1) ∧
+    RTC (active_trans conf c) S1 S2A ∧
+    RTC (internal_trans conf c) S1 S2B ⇒
+    ∃S3.
+      RTC (internal_trans conf c) S2A S3 ∧
+      RTC (active_trans conf c) S2B S3
+Proof
+  metis_tac[internal_active_comm]
+QED
+
+(* STRANS COMMUTATIVITY *)
+(* General Theorem on Conditions *)
+Theorem strans_comm_cond:
+  ∀ts.
+    (* ASSUMPTIONS *)
+    (* 1. ts preserves well formedness *)
+    (∀conf c q1 N1 q2 N2.
+      RTC (ts conf c) (q1,N1) (q2,N2) ⇒
+      ffi_wf (c,q1,N1) ⇒
+      ffi_wf (c,q2,N2)) ∧
+    (* 2. Commutes with active_trans *)
+    (∀conf c q1 N1 q2A N2A q2B N2B.
+      ffi_wf (c,q1,N1) ∧
+      RTC (ts conf c)           (q1,N1) (q2A,N2A) ∧
+      RTC (active_trans conf c) (q1,N1) (q2B,N2B) ⇒
+      ∃q3 N3.
+        RTC (active_trans conf c) (q2A,N2A) (q3,N3) ∧
+        RTC (ts conf c)           (q2B,N2B) (q3,N3)) ∧
+    (* 3. Commutes with input_trans *)
+    (∀conf c q1 N1 q2A N2A q2B N2B rp d.
+      ffi_wf (c,q1,N1) ∧
+      RTC (ts conf c) (q1,N1) (q2A,N2A) ∧
+      input_trans conf c (q1,N1) (rp,d) (q2B,N2B) ⇒
+      ∃q3 N3.
+        input_trans conf c (q2A,N2A) (rp,d) (q3,N3) ∧
+        RTC (ts conf c) (q2B,N2B) (q3,N3)) ∧
+    (* 4. Commutes with output_trans *)
+    (∀conf c q1 N1 q2A N2A q2B N2B sp d.
+      ffi_wf (c,q1,N1) ∧
+      RTC (ts conf c) (q1,N1) (q2A,N2A) ∧
+      output_trans conf c (q1,N1) (sp,d) (q2B,N2B) ⇒
+      ∃q3 N3.
+        output_trans conf c (q2A,N2A) (sp,d) (q3,N3) ∧
+        RTC (ts conf c) (q2B,N2B) (q3,N3)) ∧
+    (* 5. Commutes with internal_trans *)
+    (∀conf c q1 N1 q2A N2A q2B N2B.
+      ffi_wf (c,q1,N1) ∧
+      RTC (ts conf c)           (q1,N1) (q2A,N2A) ∧
+      RTC (internal_trans conf c) (q1,N1) (q2B,N2B) ⇒
+      ∃q3 N3.
+        RTC (internal_trans conf c) (q2A,N2A) (q3,N3) ∧
+        RTC (ts conf c)           (q2B,N2B) (q3,N3)) ⇒
+    (* CONCLUSION *)
+    (* Commutes with strans *)
+    (∀conf c q1 N1 L q2S N2S q2T N2T.
+      ffi_wf (c,q1,N1) ∧
+      strans conf (c,q1,N1) L (c,q2S,N2S) ∧
+      RTC (ts conf c) (q1,N1) (q2T,N2T) ⇒
+      ∃q3 N3.
+        RTC (ts conf c) (q2S,N2S) (q3,N3) ∧
+        strans conf (c,q2T,N2T) L (c,q3,N3))
+Proof
+  rw[] >> Cases_on ‘L’ >>
+  fs[strans_send_equiv,strans_receive_equiv]
+  >- (‘ffi_wf (c,qi,ni1) ∧ ffi_wf (c,qi,ni2)
+       ∧ ffi_wf (c,q2S,N2S) ∧ ffi_wf (c,q2T,N2T)’
+        by metis_tac[internal_trans_pres_wf,
+                     input_trans_pres_wf,
+                     active_trans_pres_wf] >>
+      last_x_assum (K ALL_TAC) >>
+      ntac 2 (last_x_assum (drule_all_then strip_assume_tac)) >>
+      last_x_assum (K ALL_TAC) >>
+      last_x_assum (drule_all_then strip_assume_tac) >>
+      rename [‘RTC (ts conf c) (q2S,N2S) (qF,NF)’,
+              ‘RTC (active_trans conf c) (q2T,N2T) (qIE,NIE)’,
+              ‘input_trans conf c (qIE,NIE) _ (qIE2,NIE2)’] >>
+      ‘qIE2 = qIE’
+        by fs[input_trans_def] >> fs[] >>
+      MAP_EVERY qexists_tac [‘qF’,‘NF’] >> rw[] >>
+      MAP_EVERY qexists_tac [‘qIE’,‘NIE’,‘NIE2’] >> rw[])
+  >- (‘ffi_wf (c,qi1,ni) ∧ ffi_wf (c,qi2,ni)
+       ∧ ffi_wf (c,q2S,N2S) ∧ ffi_wf (c,q2T,N2T)’
+        by metis_tac[internal_trans_pres_wf,
+                     output_trans_pres_wf,
+                     active_trans_pres_wf] >>
+      last_x_assum (K ALL_TAC) >>
+      last_x_assum (drule_all_then strip_assume_tac) >>
+      last_x_assum (K ALL_TAC) >>
+      ntac 2  (last_x_assum (drule_all_then strip_assume_tac)) >>
+      rename [‘RTC (ts conf c) (q2S,N2S) (qF,NF)’,
+              ‘RTC (active_trans conf c) (q2T,N2T) (qIE,NIE)’,
+              ‘output_trans conf c (qIE,NIE) _ (qIE2,NIE2)’] >>
+      ‘NIE2 = NIE’
+        by fs[output_trans_def] >> fs[] >>
+      MAP_EVERY qexists_tac [‘qF’,‘NF’] >> rw[] >>
+      MAP_EVERY qexists_tac [‘qIE’,‘qIE2’,‘NIE’] >> rw[])
+QED
+
+(* Application to Specific Pieces *)
+(* -- internal/strans commutativity *)
+Theorem internal_strans_comm:
+  ∀conf c q1 N1 L q2S N2S q2T N2T.
+    ffi_wf (c,q1,N1) ∧
+    strans conf (c,q1,N1) L (c,q2S,N2S) ∧
+    RTC (internal_trans conf c) (q1,N1) (q2T,N2T) ⇒
+    ∃q3 N3.
+      RTC (internal_trans conf c) (q2S,N2S) (q3,N3) ∧
+      strans conf (c,q2T,N2T) L (c,q3,N3)
+Proof
+  qspec_then ‘internal_trans’ assume_tac strans_comm_cond >>
+  qmatch_asmsub_abbrev_tac ‘A ⇒ B’ >>
+  ‘A’ suffices_by fs[] >>
+  qpat_x_assum ‘A ⇒ B’ (K ALL_TAC) >>
+  MAP_EVERY qunabbrev_tac [‘A’,‘B’] >>
+  rw[GSYM pairTheory.FORALL_PROD,
+     GSYM pairTheory.EXISTS_PROD]
+  >- metis_tac[internal_trans_pres_wf]
+  >- metis_tac[internal_active_comm]
+  >- metis_tac[internal_send_comm]
+  >- metis_tac[internal_rec_comm]
+  >- metis_tac[internal_internal_comm]
+QED
+
+(* -- active/strans commutativity *)
+Theorem active_strans_comm:
+  ∀conf c q1 N1 L q2S N2S q2T N2T.
+    ffi_wf (c,q1,N1) ∧
+    strans conf (c,q1,N1) L (c,q2S,N2S) ∧
+    RTC (active_trans conf c) (q1,N1) (q2T,N2T) ⇒
+    ∃q3 N3.
+      RTC (active_trans conf c) (q2S,N2S) (q3,N3) ∧
+      strans conf (c,q2T,N2T) L (c,q3,N3)
+Proof
+  qspec_then ‘active_trans’ assume_tac strans_comm_cond >>
+  qmatch_asmsub_abbrev_tac ‘A ⇒ B’ >>
+  ‘A’ suffices_by fs[] >>
+  qpat_x_assum ‘A ⇒ B’ (K ALL_TAC) >>
+  MAP_EVERY qunabbrev_tac [‘A’,‘B’] >>
+  rw[GSYM pairTheory.FORALL_PROD,
+     GSYM pairTheory.EXISTS_PROD]
+  >- metis_tac[active_trans_pres_wf]
+  >- metis_tac[active_active_comm]
+  >- metis_tac[active_send_comm]
+  >- metis_tac[active_rec_comm]
+  >- metis_tac[active_internal_comm]
+QED
+
+val _ = export_theory ();
