projection/proofs/ffi/comms_ffi_consScript.sml
@@ -1,0 +1,241 @@
+open HolKernel boolLib Parse bossLib;
+open relationTheory;
+open payloadSemanticsTheory;
+open comms_ffi_modelTheory;
+
+val _ = new_theory "comms_ffi_cons";
+
+(* BUILDING BLOCK TRANSITIONS *)
+(* Internal Transition *)
+Definition internal_trans_def:
+  internal_trans conf (c:proc) (q1:queues,n1:network) (q2:queues,n2:network) ⇔
+    trans conf n1 LTau n2 ∧ q1 = q2
+End
+
+(* Emission Transition *)
+Definition emit_trans_def:
+  emit_trans conf (c:proc) (q1:queues,n1:network) (q2:queues,n2:network) ⇔
+    ∃sp d .
+      trans conf n1 (LSend sp d c) n2 ∧
+      q2 = qpush q1 sp d
+End
+
+(* Emission or Internal Transition *)
+Definition active_trans_def:
+  active_trans conf c (q1,n1) (q2,n2) ⇔
+    internal_trans conf c (q1,n1) (q2,n2) ∨
+    emit_trans     conf c (q1,n1) (q2,n2)
+End
+
+(* Input Transition *)
+Definition input_trans_def:
+  input_trans conf c (q1,n1) (rp,d) (q2,n2) ⇔
+    trans conf n1 (LReceive c d rp) n2 ∧
+    q2 = q1
+End
+
+(* Output Transition *)
+Definition output_trans_def:
+  output_trans conf c (q1,n1) (sp,d) (q2,n2) ⇔
+    (n1 = n2) ∧
+    (q1 = q2 |+ (sp,d::(qlk q2 sp))) ∧
+    (q2 = q2 |+ (sp,qlk q2 sp))
+End
+
+
+(* GENERAL CONSTRUCTION FACTS *)
+(* Front Addition *)
+Theorem strans_front_construct:
+  ∀conf q1 n1 qi ni q2 n2 c L.
+    RTC (active_trans conf c) (q1,n1) (qi,ni) ∧
+    strans conf (c,qi,ni) L (c,q2,n2) ⇒
+    strans conf (c,q1,n1) L (c,q2,n2)
+Proof
+  rpt gen_tac >>
+  ‘∀S1 S2.
+    RTC (active_trans conf c) S1 S2 ⇒
+      (λ(q1,n1) (qi,ni).
+        strans conf (c,qi,ni) L (c,q2,n2) ⇒
+        strans conf (c,q1,n1) L (c,q2,n2)) S1 S2’
+    suffices_by (disch_then (qspecl_then [‘(q1,n1)’,‘(qi,ni)’] assume_tac) >>
+                 rw[] >> fs[]) >>
+  ho_match_mp_tac RTC_INDUCT >>
+  rw[]
+  >- (Cases_on ‘S1’ >> rw[])
+  >- (rename [‘active_trans conf c S1 S1B’] >>
+      Cases_on ‘S1’ >> Cases_on ‘S1B’ >> Cases_on ‘S2’ >>
+      rw[] >> fs[active_trans_def,internal_trans_def,emit_trans_def]
+      >- metis_tac[strans_rules]
+      >- metis_tac[strans_rules])
+QED
+
+(* Back Addition *)
+Theorem strans_back_construct:
+  ∀conf q1 n1 qi ni q2 n2 c L.
+    strans conf (c,q1,n1) L (c,qi,ni) ∧
+    RTC (internal_trans conf c) (qi,ni) (q2,n2)     ⇒
+    strans conf (c,q1,n1) L (c,q2,n2)
+Proof
+  rpt gen_tac >>
+  ‘∀S1 S2.
+    RTC (internal_trans conf c) S1 S2 ⇒
+      (λ(qi,ni) (q2,n2).
+        strans conf (c,q1,n1) L (c,qi,ni) ⇒
+        strans conf (c,q1,n1) L (c,q2,n2)) S1 S2’
+    suffices_by (disch_then (qspecl_then [‘(qi,ni)’,‘(q2,n2)’] assume_tac) >>
+                 rw[] >> fs[]) >>
+  ho_match_mp_tac RTC_INDUCT >>
+  rw[]
+  >- (Cases_on ‘S1’ >> rw[])
+  >- (rename [‘internal_trans conf c S1 S1B’] >>
+      Cases_on ‘S1’ >> Cases_on ‘S1B’ >> Cases_on ‘S2’ >>
+      rw[] >> fs[internal_trans_def] >>
+      rfs[] >>
+      ‘strans conf (c,q1,n1) L (c,q',r')’
+        suffices_by rw[] >>
+      metis_tac[strans_rules])
+QED
+
+
+(* SEND CONSTRUCTION/DECONSTRUCTION *)
+(* Pulling apart a send operation *)
+Theorem strans_send_deconstruct:
+  ∀conf c q1 q2 n1 d rp n2.
+    strans conf (c,q1,n1) (ASend rp d) (c,q2,n2) ⇒
+    ∃ni1 ni2 qi.
+      RTC (active_trans conf c) (q1,n1) (qi,ni1) ∧
+      input_trans conf c (qi,ni1) (rp,d) (qi,ni2) ∧
+      RTC (internal_trans conf c) (qi,ni2) (q2,n2)
+Proof
+  Induct_on ‘strans’ >> rw[]
+  >- (MAP_EVERY qexists_tac [‘ni1’,‘ni2’,‘qi’] >>
+      rename [‘trans conf N LTau Np’] >>
+      ‘RTC (active_trans conf c) (q,N) (q,Np)’
+        suffices_by metis_tac[RTC_TRANSITIVE,transitive_def] >>
+      irule RTC_SINGLE >>
+      rw[active_trans_def,internal_trans_def])
+  >- (MAP_EVERY qexists_tac [‘ni1’,‘ni2’,‘qi’] >>
+      rename [‘trans conf N LTau Np’,
+              ‘RTC _ (qi,ni2) (qf,N)’] >>
+      ‘RTC (internal_trans conf c) (qf,N) (qf,Np)’
+        suffices_by metis_tac[RTC_TRANSITIVE,transitive_def] >>
+      irule RTC_SINGLE >>
+      rw[active_trans_def,internal_trans_def])
+  >- (MAP_EVERY qexists_tac [‘ni1’,‘ni2’,‘qi’] >>
+      rename [‘trans conf N (LSend _ _ _) Np’] >>
+      ‘RTC (active_trans conf c) (q,N) (qpush q sp d,Np)’
+        suffices_by metis_tac[RTC_TRANSITIVE,transitive_def] >>
+      irule RTC_SINGLE >>
+      rw[active_trans_def,emit_trans_def] >>
+      DISJ2_TAC >>
+      metis_tac[])
+  >- (metis_tac[RTC_RULES,input_trans_def])
+QED 
+
+(* Constructing a send operation *)
+Theorem strans_send_construct:
+  ∀conf q1 n1 qi ni1 c d rp ni2 q2 n2.
+    RTC (active_trans conf c) (q1,n1) (qi,ni1) ∧
+    input_trans conf c (qi,ni1) (rp,d) (qi,ni2) ∧
+    RTC (internal_trans conf c) (qi,ni2) (q2,n2) ⇒
+      strans conf (c,q1,n1) (ASend rp d) (c,q2,n2)
+Proof
+  metis_tac[input_trans_def, strans_rules,
+            strans_front_construct,strans_back_construct]
+QED 
+
+(* Send Label Equivalence *)
+Theorem strans_send_equiv:
+  ∀conf q1 n1 c d rp q2 n2.
+    strans conf (c,q1,n1) (ASend rp d) (c,q2,n2) ⇔
+    ∃qi ni1 ni2.
+      RTC (active_trans conf c) (q1,n1) (qi,ni1) ∧
+      input_trans conf c (qi,ni1) (rp,d) (qi,ni2) ∧
+      RTC (internal_trans conf c) (qi,ni2) (q2,n2)
+Proof
+  metis_tac[strans_send_deconstruct,strans_send_construct]
+QED
+
+
+(* RECEIVE CONSTRUCTION/DECONSTRUCTION *)
+(* Pulling apart a receive operation *)
+Theorem strans_receive_deconstruct:
+  ∀conf c q1 q2 n1 d sp n2.
+    strans conf (c,q1,n1) (ARecv sp d) (c,q2,n2) ⇒
+    ∃qi1 qi2 ni.
+      RTC (active_trans conf c) (q1,n1) (qi1,ni) ∧
+      output_trans conf c (qi1,ni) (sp,d) (qi2,ni) ∧
+      RTC (internal_trans conf c) (qi2,ni) (q2,n2)
+Proof
+  Induct_on ‘strans’ >> rw[]
+  >- (rename1 ‘qlk q ms = mc::tl’ >>
+      MAP_EVERY qexists_tac [‘q |+ (ms,mc::tl)’,‘q |+ (ms,tl)’,‘N’] >>
+      rw[qlk_def,fget_def,finite_mapTheory.FLOOKUP_DEF,output_trans_def] >>
+      ‘q |+ (ms,mc:: tl) = q’
+        suffices_by (rw[] >> metis_tac[RC_DEF]) >>
+      irule finite_mapTheory.FUPDATE_ELIM >>
+      fs[qlk_def,fget_def,finite_mapTheory.FLOOKUP_DEF] >>
+      Cases_on ‘ms ∈ FDOM q’ >> fs[])
+  >- (rename [‘trans conf NA LTau NB’,
+              ‘RTC _ (qA,NB) (qC,NCD)’,
+              ‘output_trans conf c (qC,NCD) (sp,d) (qD,NCD)’,
+              ‘RTC _ (qD,NCD) (qE,NE)’] >>
+      MAP_EVERY qexists_tac [‘qC’,‘qD’,‘NCD’] >>
+      fs[output_trans_def] >>
+      ‘RTC (active_trans conf c) (qA,NA) (qA,NB)’
+        suffices_by metis_tac[RTC_TRANSITIVE,transitive_def] >>
+      irule RTC_SINGLE >>
+      rw[active_trans_def,internal_trans_def])
+  >- (rename [‘RTC _ (qA,NA) (qB,NB)’,
+              ‘output_trans conf c (qB,NB) (sp,d) (qC,NC)’,
+              ‘RTC _ (qC,NC) (qDE,ND)’,
+              ‘trans conf ND LTau NE’] >>
+      MAP_EVERY qexists_tac [‘qB’,‘qC’,‘NC’] >>
+      fs[output_trans_def] >>
+      ‘RTC (internal_trans conf c) (qDE,ND) (qDE,NE)’
+        suffices_by metis_tac[RTC_TRANSITIVE,transitive_def] >>
+      irule RTC_SINGLE >>
+      rw[internal_trans_def])
+  >- (rename [‘trans conf NA (LSend sp d c) NB’,
+              ‘RTC _ (qpush qA sp d,NB) (qC,NCD)’,
+              ‘output_trans conf c (qC,NCD) (sp2,d2) (qD,NCD)’,
+              ‘RTC _ (qD,NCD) (qE,NE)’] >>
+      MAP_EVERY qexists_tac [‘qC’,‘qD’,‘NCD’] >>
+      fs[output_trans_def] >>
+      ‘RTC (active_trans conf c) (qA,NA) (qpush qA sp d,NB)’
+        suffices_by metis_tac[RTC_TRANSITIVE,transitive_def] >>
+      irule RTC_SINGLE >>
+      rw[active_trans_def,emit_trans_def] >>
+      metis_tac[])
+QED 
+
+(* Constructing a receive operation *)
+Theorem strans_receive_construct:
+  ∀conf c q1 q2 n1 d sp n2 qi1 qi2 ni.
+    RTC (active_trans conf c) (q1,n1) (qi1,ni) ∧
+    output_trans conf c (qi1,ni) (sp,d) (qi2,ni) ∧
+    RTC (internal_trans conf c) (qi2,ni) (q2,n2) ⇒
+  	strans conf (c,q1,n1) (ARecv sp d) (c,q2,n2)
+Proof
+  rw[] >>
+  ‘strans conf (c,qi1,ni) (ARecv sp d) (c,qi2,ni)’
+    suffices_by metis_tac[strans_front_construct,strans_back_construct] >>
+  ‘(qlk qi1 sp = d::(qlk qi2 sp)) ∧
+   (qi2 = qi1 |+ (sp,qlk qi2 sp))’
+    by (fs[output_trans_def,qlk_def,fget_def,finite_mapTheory.FLOOKUP_UPDATE]) >>
+  metis_tac[strans_rules]
+QED 
+
+(* Receive Label Equivalence *)
+Theorem strans_receive_equiv:
+  ∀conf c q1 q2 n1 d sp n2.
+    strans conf (c,q1,n1) (ARecv sp d) (c,q2,n2) ⇔
+    ∃qi1 qi2 ni.
+      RTC (active_trans conf c) (q1,n1) (qi1,ni) ∧
+      output_trans conf c (qi1,ni) (sp,d) (qi2,ni) ∧
+      RTC (internal_trans conf c) (qi2,ni) (q2,n2)
+Proof
+  metis_tac[strans_receive_deconstruct,strans_receive_construct]
+QED
+
+val _ = export_theory ();
