projection/proofs/ffi/comms_ffi_propsScript.sml
@@ -1,0 +1,396 @@
+open HolKernel boolLib Parse bossLib;
+open optionTheory
+     relationTheory
+     listTheory
+     rich_listTheory;
+open ffiTheory;
+open bisimulationTheory
+     payloadSemanticsTheory
+     payloadLangTheory
+     payloadPropsTheory
+     comms_ffi_modelTheory
+     comms_ffi_consTheory;
+
+val _ = new_theory "comms_ffi_props";
+
+(* FUNDAMENTAL FFI STATE INVARIANTS/PROPERTIES *)
+(* Process Number *)
+Theorem strans_pres_pnum:
+  ∀conf s1 L s2.
+    strans conf s1 L s2 ⇒
+      FST s1 = FST s2
+Proof
+  rw[Once strans_cases] >>
+  simp[]
+QED
+
+(* Message Queue *)
+Theorem strans_queue_pres:
+  ∀conf P Q1 N1 D M Q2 N2.
+    strans conf (P,Q1,N1) (ASend D M) (P,Q2,N2) ⇒
+      ∀sp.
+        isPREFIX (qlk Q1 sp) (qlk Q2 sp)
+Proof
+  Induct_on ‘strans’ >> rw[] >>
+  metis_tac[IS_PREFIX_TRANS,qpush_prefix]
+QED
+
+(* Message Queue Irrelevance *)
+(* -- Lemma about queue growth *)
+Theorem active_trans_queue_expand:
+  ∀conf c q1 n1 q2 n2.
+    RTC (active_trans conf c) (q1,n1) (q2,n2) ⇒
+    ∀sp.
+      isPREFIX (qlk q1 sp) (qlk q2 sp)
+Proof
+  rw[] >>
+  ‘∀s1 s2. RTC (active_trans conf c) s1 s2 ⇒
+           (λ(q1,n1) (q2,n2).
+              ∀sp.
+                isPREFIX (qlk q1 sp) (qlk q2 sp)) s1 s2’
+    suffices_by (rw[] >>
+                 first_x_assum (qspecl_then [‘(q1,n1)’,‘(q2,n2)’] assume_tac) >>
+                 rfs[]) >>
+  ho_match_mp_tac RTC_INDUCT >>
+  first_x_assum (K ALL_TAC) >>
+  rw[]
+  >- (PairCases_on ‘s1’ >> rw[])
+  >- (rename [‘_ _ s1 s2’,‘_ s2 s3’] >>
+      PairCases_on  ‘s1’ >> PairCases_on ‘s2’ >>
+      PairCases_on ‘s3’ >>
+      fs[active_trans_def,internal_trans_def,emit_trans_def] >>
+      rw[] >>
+      last_x_assum (K ALL_TAC) >>
+      metis_tac[IS_PREFIX_TRANS,qpush_prefix])
+QED
+
+(* -- Helper lemmas about queue irrelevance *)
+Definition qsame_def:
+  qsame q1 q2 ⇔ ∀sp. qlk q1 sp = qlk q2 sp
+End
+
+(* -- -- Internal Transition *)
+Theorem qsame_irrel_internal:
+  ∀conf c q1 q1M N1 q2 N2.
+    RTC (internal_trans conf c) (q1,N1) (q2,N2) ⇒
+    qsame q1 q1M ⇒
+    ∃q2M.
+      RTC (internal_trans conf c) (q1M,N1) (q2M,N2) ∧
+      qsame q2 q2M
+Proof
+  simp[qsame_def] >>
+  rpt gen_tac >>
+  ‘∀s1 s2.
+    RTC (internal_trans conf c) s1 s2 ⇒
+    (λ(q1,N1) (q2,N2).
+      ∀q1M.
+        (∀sp. qlk q1 sp = qlk q1M sp) ⇒
+        ∃q2M.
+          RTC (internal_trans conf c) (q1M,N1) (q2M,N2) ∧
+          (∀sp. qlk q2 sp = qlk q2M sp)) s1 s2’
+    suffices_by (rw[pairTheory.FORALL_PROD] >>
+                 metis_tac[]) >>
+  Induct_on ‘RTC’ >> rw[]
+  >- (PairCases_on ‘s1’ >> rw[] >>
+      qexists_tac ‘q1M’ >> metis_tac[RTC_REFL]) >>
+  rename1 ‘internal_trans conf c s1 sI’ >>
+  MAP_EVERY PairCases_on [‘s1’,‘sI’,‘s2’] >>
+  fs[] >> rw[] >>
+  ‘∃sI0M.
+    internal_trans conf c (q1M,s11) (sI0M,sI1) ∧
+    (∀sp. qlk sI0 sp = qlk sI0M sp)’
+    suffices_by metis_tac[RTC_TRANSITIVE,transitive_def,RTC_SINGLE] >>
+  metis_tac[internal_trans_def]
+QED
+
+(* -- -- Active Transition *)
+Theorem qsame_irrel_active:
+  ∀conf c q1 q1M N1 q2 N2.
+    RTC (active_trans conf c) (q1,N1) (q2,N2) ⇒
+    qsame q1 q1M ⇒
+    ∃q2M.
+      RTC (active_trans conf c) (q1M,N1) (q2M,N2) ∧
+      qsame q2 q2M
+Proof
+  simp[qsame_def] >>
+  rpt gen_tac >>
+  ‘∀s1 s2.
+    RTC (active_trans conf c) s1 s2 ⇒
+    (λ(q1,N1) (q2,N2).
+      ∀q1M.
+        (∀sp. qlk q1 sp = qlk q1M sp) ⇒
+        ∃q2M.
+          RTC (active_trans conf c) (q1M,N1) (q2M,N2) ∧
+          (∀sp. qlk q2 sp = qlk q2M sp)) s1 s2’
+    suffices_by (rw[pairTheory.FORALL_PROD] >>
+                 metis_tac[]) >>
+  Induct_on ‘RTC’ >> rw[]
+  >- (PairCases_on ‘s1’ >> rw[] >>
+      qexists_tac ‘q1M’ >> metis_tac[RTC_REFL]) >>
+  rename1 ‘active_trans conf c s1 sI’ >>
+  MAP_EVERY PairCases_on [‘s1’,‘sI’,‘s2’] >>
+  fs[] >> rw[] >>
+  ‘∃sI0M.
+    active_trans conf c (q1M,s11) (sI0M,sI1) ∧
+    (∀sp. qlk sI0 sp = qlk sI0M sp)’
+    suffices_by metis_tac[RTC_TRANSITIVE,transitive_def,RTC_SINGLE] >>
+  last_x_assum assume_tac >>
+  ntac 2 (last_x_assum (K ALL_TAC)) >>
+  pop_assum (assume_tac o REWRITE_RULE [active_trans_def]) >>
+  fs[emit_trans_def,internal_trans_def]
+  >- metis_tac[active_trans_def,internal_trans_def] >>
+  qexists_tac ‘qpush q1M sp d’ >>
+  fs[active_trans_def,emit_trans_def] >> rw[]
+  >- metis_tac[] >>
+  fs[qpush_def,qlk_def,fget_def] >>
+  metis_tac[finite_mapTheory.FLOOKUP_UPDATE]
+QED
+
+(* -- -- Input Transition *)
+Theorem qsame_irrel_send:
+  ∀conf c q1 q1M N1 rp d q2 N2.
+    input_trans conf c (q1,N1) (rp,d) (q2,N2) ⇒
+    qsame q1 q1M ⇒
+    ∃q2M.
+      input_trans conf c (q1M,N1) (rp,d) (q2M,N2) ∧
+      qsame q2 q2M
+Proof
+  rw[qsame_def,input_trans_def]
+QED
+
+(* -- -- Receive Transition *)
+Theorem qsame_irrel_receive:
+  ∀conf c q1 q1M N1 rp d q2 N2.
+    output_trans conf c (q1,N1) (sp,d) (q2,N2) ⇒
+    qsame q1 q1M ⇒
+    ∃q2M.
+      output_trans conf c (q1M,N1) (sp,d) (q2M,N2) ∧
+      qsame q2 q2M
+Proof
+  rw[qsame_def,output_trans_def] >>
+  qexists_tac ‘q1M |+ (sp,qlk q2 sp)’ >>
+  rw[finite_mapTheory.FLOOKUP_EXT,FUN_EQ_THM]
+  >- (reverse (Cases_on ‘x = sp’)
+      >- metis_tac[finite_mapTheory.FLOOKUP_UPDATE] >>
+      rw[finite_mapTheory.FLOOKUP_UPDATE,qlk_def,
+         fget_def] >>
+      pop_assum (qspec_then ‘sp’ assume_tac) >>
+      fs[finite_mapTheory.FLOOKUP_UPDATE,qlk_def,fget_def] >>
+      Cases_on ‘FLOOKUP q1M sp’ >> fs[])
+  >- (reverse (Cases_on ‘x = sp’)
+      >- metis_tac[finite_mapTheory.FLOOKUP_UPDATE] >>
+      rw[finite_mapTheory.FLOOKUP_UPDATE,qlk_def,
+         fget_def])
+  >- (rename1 ‘qlk q2 x = qlk _ x’ >>
+      fs[qlk_def,fget_def] >>
+      reverse (Cases_on ‘x = sp’)
+      >- metis_tac[finite_mapTheory.FLOOKUP_UPDATE] >>
+      rw[finite_mapTheory.FLOOKUP_UPDATE])
+QED
+
+(* Network Properties *)
+(* -- Contained Nodes *)
+Definition ffi_has_node_def:
+  ffi_has_node nd (P,Q,N) =
+    net_has_node N nd
+End
+
+Theorem strans_pres_nodes:
+  ∀conf s0 l s1.
+    strans conf s0 l s1 ⇒
+      (∀nd. ffi_has_node nd s0 ⇔ ffi_has_node nd s1)
+Proof
+  Induct_on ‘strans’ >> rw[ffi_has_node_def] >>
+  metis_tac[trans_pres_nodes]
+QED
+
+(* -- Wellformedness *)
+Definition ffi_wf_def:
+  ffi_wf (c,q,n) ⇔ net_wf n ∧ ¬net_has_node n c
+End
+
+Theorem strans_pres_wf:
+  ∀conf s1 L s2.
+    strans conf s1 L s2 ⇒
+      (ffi_wf s1 ⇔ ffi_wf s2)
+Proof
+  Induct_on ‘strans’ >> rw[ffi_wf_def] >>
+  metis_tac[trans_pres_nodes,trans_pres_wf]
+QED
+
+Theorem internal_trans_pres_wf:
+  ∀conf c q1 N1 q2 N2.
+    RTC (internal_trans conf c) (q1,N1) (q2,N2) ⇒
+    ffi_wf (c,q1,N1) ⇒
+    ffi_wf (c,q2,N2)
+Proof
+  rpt gen_tac >>
+  qmatch_goalsub_abbrev_tac ‘RTC _ S1 S2’ >>
+  MAP_EVERY qid_spec_tac [‘S1’,‘S2’] >>
+  Induct_on ‘RTC’ >> rw[] >>
+  rename1 ‘ffi_wf (c,SK) ⇒ ffi_wf (c,SU)’ >>
+  ‘ffi_wf (c,SK)’
+    suffices_by rw[] >>
+  rename1 ‘internal_trans conf c SB SK’ >>
+  MAP_EVERY PairCases_on [‘SB’,‘SK’] >>
+  fs[internal_trans_def,ffi_wf_def] >>
+  metis_tac[trans_pres_nodes,trans_pres_wf]
+QED 
+
+Theorem emit_trans_pres_wf:
+  ∀conf c q1 N1 q2 N2.
+    RTC (emit_trans conf c) (q1,N1) (q2,N2) ⇒
+    ffi_wf (c,q1,N1) ⇒
+    ffi_wf (c,q2,N2)
+Proof
+  rpt gen_tac >>
+  qmatch_goalsub_abbrev_tac ‘RTC _ S1 S2’ >>
+  MAP_EVERY qid_spec_tac [‘S1’,‘S2’] >>
+  Induct_on ‘RTC’ >> rw[] >>
+  rename1 ‘ffi_wf (c,SK) ⇒ ffi_wf (c,SU)’ >>
+  ‘ffi_wf (c,SK)’
+    suffices_by rw[] >>
+  rename1 ‘emit_trans conf c SB SK’ >>
+  MAP_EVERY PairCases_on [‘SB’,‘SK’] >>
+  fs[emit_trans_def,ffi_wf_def] >>
+  metis_tac[trans_pres_nodes,trans_pres_wf]
+QED 
+
+Theorem active_trans_pres_wf:
+  ∀conf c q1 N1 q2 N2.
+    RTC (active_trans conf c) (q1,N1) (q2,N2) ⇒
+    ffi_wf (c,q1,N1) ⇒
+    ffi_wf (c,q2,N2)
+Proof
+  rpt gen_tac >>
+  qmatch_goalsub_abbrev_tac ‘RTC _ S1 S2’ >>
+  MAP_EVERY qid_spec_tac [‘S1’,‘S2’] >>
+  Induct_on ‘RTC’ >> rw[] >>
+  rename1 ‘ffi_wf (c,SK) ⇒ ffi_wf (c,SU)’ >>
+  ‘ffi_wf (c,SK)’
+    suffices_by rw[] >>
+  rename1 ‘active_trans conf c SB SK’ >>
+  MAP_EVERY PairCases_on [‘SB’,‘SK’] >>
+  fs[active_trans_def,internal_trans_def,
+     emit_trans_def,ffi_wf_def] >>
+  metis_tac[trans_pres_nodes,trans_pres_wf]
+QED 
+
+Theorem input_trans_pres_wf:
+  ∀conf c q1 N1 rp d q2 N2.
+    input_trans conf c (q1,N1) (rp,d) (q2,N2) ⇒
+    ffi_wf (c,q1,N1) ⇒
+    ffi_wf (c,q2,N2)
+Proof
+  rw[input_trans_def,ffi_wf_def] >>
+  metis_tac[trans_pres_nodes,trans_pres_wf]
+QED 
+
+Theorem output_trans_pres_wf:
+  ∀conf c q1 N1 sp d q2 N2.
+    output_trans conf c (q1,N1) (sp,d) (q2,N2) ⇒
+    ffi_wf (c,q1,N1) ⇒
+    ffi_wf (c,q2,N2)
+Proof
+  rw[output_trans_def,ffi_wf_def] >>
+  metis_tac[trans_pres_nodes,trans_pres_wf]
+QED 
+
+
+(* FFI STATE COMMUNICATION PROPERTIES *)
+(* Send Validity Checks *)
+(* -- Destination *)
+Definition valid_send_dest_def:
+  valid_send_dest dest ffiSt = ((FST ffiSt ≠ dest) ∧ (ffi_has_node dest ffiSt))
+End
+(* -- Call Format *)
+Definition valid_send_call_format_def:
+  valid_send_call_format conf dest s c bytes =
+    ((s = "send") ∧ (c = dest) ∧ (LENGTH bytes = SUC conf.payload_size))
+End
+(* -- Event Format *)
+Definition valid_send_event_format_def:
+  valid_send_event_format conf dest event =
+    case event of
+      IO_event n d c =>
+         (valid_send_call_format conf dest n d (MAP FST c) ∧
+          (MAP FST c = MAP SND c))
+End
+
+(* Send Properties *)
+(* -- Sufficient Sending Conditions *)
+Theorem strans_send_cond:
+  ∀S1 dest conf.
+    valid_send_dest dest S1 ⇒
+    (∀bytes. ∃S2.
+      strans conf S1 (ASend dest bytes) S2)
+Proof
+  rw[] >> Cases_on ‘S1’ >> qmatch_goalsub_rename_tac ‘(P,R)’ >>
+  Cases_on ‘R’  >> qmatch_goalsub_rename_tac ‘(P,Q1,N1)’ >>
+  ‘∃N2. trans conf N1 (LReceive P bytes dest) N2’
+    suffices_by metis_tac[strans_rules] >>
+  fs[valid_send_dest_def,ffi_has_node_def] >>
+  metis_tac[trans_receive_cond]
+QED
+(* -- Necessary Sending Conditions *)
+Theorem strans_dest_check:
+  ∀S1 dest conf.
+    (∃bytes S2.
+      strans conf S1 (ASend dest bytes) S2) ⇒
+    valid_send_dest dest S1
+Proof
+  Induct_on ‘strans’ >>
+  rw[valid_send_dest_def,ffi_has_node_def] >>
+  metis_tac[trans_pres_nodes,trans_receive_cond]
+QED
+
+
+(* COMPLEX FFI STATE INVARIANTS *)
+(* Basic FFI State Invariant Definition *)
+Definition ffi_accepts_rel_def:
+  ffi_accepts_rel stpred pred oracle =
+  ∀st s conf bytes.
+    stpred st.ffi_state ∧ st.oracle = oracle ∧ pred s conf bytes ⇒
+    ∃ffi. st.oracle s st.ffi_state conf bytes = Oracle_return ffi bytes ∧
+          stpred ffi
+End
+
+(* Basic FFI Send Invariant *)
+Theorem send_invariant:
+  ∀ conf l.
+    ffi_accepts_rel (valid_send_dest l) (valid_send_call_format conf l) (comms_ffi_oracle conf)
+Proof
+  rw[valid_send_dest_def,ffi_accepts_rel_def,valid_send_call_format_def,
+     comms_ffi_oracle_def,ffi_send_def] >>
+  DEEP_INTRO_TAC some_intro >>
+  qmatch_goalsub_abbrev_tac ‘strans _ s _’ >>
+  first_x_assum (K ALL_TAC) >>
+  qpat_x_assum ‘_ = comms_ffi_oracle conf’ (K ALL_TAC) >>
+  rw[]
+  >- (rename1 ‘strans _ s _ s2’ >>
+      Cases_on ‘s’ >> Cases_on ‘s2’ >>
+      metis_tac[strans_pres_pnum])
+  >- (rename1 ‘strans _ s _ s2’ >>
+      Cases_on ‘s’ >> Cases_on ‘s2’ >>
+      metis_tac[strans_pres_nodes])
+  >- metis_tac[valid_send_dest_def,strans_send_cond]
+QED
+
+(* Complex FFI State Invariant Definition *)
+Definition ffi_laccepts_def:
+  (ffi_laccepts 0 oracle ipred mpred fpred st =
+    ∀s conf bytes.
+      ipred s conf bytes ⇒
+      ∃ffi nbytes.
+          (oracle s st conf bytes = Oracle_return ffi nbytes) ∧
+          (fpred nbytes)) ∧
+  (ffi_laccepts (SUC n) oracle ipred mpred fpred st =
+    ∀s conf bytes.
+      ipred s conf bytes ⇒
+        ∃ffi nbytes.
+          (oracle s st conf bytes = Oracle_return ffi nbytes) ∧
+          (mpred nbytes) ∧
+          (ffi_laccepts n oracle ipred mpred fpred ffi))
+End
+
+val _ = export_theory ();
