projection/proofs/ffi/confluenceScript.sml
@@ -1,0 +1,155 @@
+open  HolKernel
+      boolLib
+      bossLib
+      relationTheory;
+
+val _ = new_theory "confluence";
+
+Theorem diam_to_srtc_diam:
+  ∀tsA tsB wfP.
+    (* ASSUMPTIONS *)
+    (* 1. wfP is preserved by tsA and tsB *)
+    (∀x y.
+      wfP x ∧ tsA x y ⇒ wfP y) ∧
+    (∀x y.
+      wfP x ∧ tsB x y ⇒ wfP y) ∧
+    (* 2. tsA and tsB have diamond on wfP states *)
+    (∀S1 S2A S2B.
+      wfP S1 ∧
+      tsA S1 S2A ∧
+      tsB S1 S2B ⇒
+      ∃S3.
+        tsB S2A S3 ∧
+        tsA S2B S3) ⇒
+    (* CONCLUSION *)
+    (* tsA and tsB have semi-RTC diamond on wfP states *)
+    (∀S1 S2A S2B.
+      wfP S1 ∧
+      RTC tsA S1 S2A ∧
+      tsB S1 S2B ⇒
+      ∃S3.
+        tsB S2A S3 ∧
+        RTC tsA S2B S3)
+Proof
+  rw[] >>
+  pop_assum mp_tac >>
+  qpat_x_assum ‘wfP S1’ mp_tac >>
+  pop_assum mp_tac >>
+  MAP_EVERY qid_spec_tac [‘S1’,‘S2A’,‘S2B’] >>
+  Induct_on ‘RTC’ >> rw[]
+  >- metis_tac[RC_DEF,RTC_REFL] >>
+  rename [‘wfP S1’,‘tsA S1 SI’,‘RTC tsA SI S2A’,‘tsB S1 S2B’] >>
+  ntac 2 (last_x_assum assume_tac) >>
+  last_x_assum (drule_all_then strip_assume_tac) >>
+  ‘wfP SI’
+    by metis_tac[] >>
+  fs[] >>
+  last_x_assum (drule_all_then strip_assume_tac) >>
+  metis_tac[RTC_TRANSITIVE,transitive_def,RTC_SINGLE]
+QED
+
+Theorem rc_diam_to_srtc_diam:
+  ∀tsA tsB wfP.
+    (* ASSUMPTIONS *)
+    (* 1. wfP is preserved by tsA and tsB *)
+    (∀x y.
+      wfP x ∧ tsA x y ⇒ wfP y) ∧
+    (∀x y.
+      wfP x ∧ tsB x y ⇒ wfP y) ∧
+    (* 2. tsA and tsB have RC diamond on wfP states *)
+    (∀S1 S2A S2B.
+      wfP S1 ∧
+      tsA S1 S2A ∧
+      tsB S1 S2B ⇒
+      ∃S3.
+        RC tsB S2A S3 ∧
+        RC tsA S2B S3) ⇒
+    (* CONCLUSION *)
+    (* tsA and tsB have semi-RTC diamond on wfP states *)
+    (∀S1 S2A S2B.
+      wfP S1 ∧
+      RTC tsA S1 S2A ∧
+      tsB S1 S2B ⇒
+      ∃S3.
+        RC tsB S2A S3 ∧
+        RTC tsA S2B S3)
+Proof
+  rw[] >>
+  pop_assum mp_tac >>
+  qpat_x_assum ‘wfP S1’ mp_tac >>
+  pop_assum mp_tac >>
+  MAP_EVERY qid_spec_tac [‘S1’,‘S2A’,‘S2B’] >>
+  Induct_on ‘RTC’ >> rw[]
+  >- metis_tac[RC_DEF,RTC_REFL] >>
+  rename[‘tsA S1 SI’,‘tsB S1 S2B’] >>
+  ntac 2 (last_x_assum assume_tac) >>
+  last_x_assum (drule_all_then strip_assume_tac) >>
+  rpt (qpat_x_assum ‘RC _ _ _’ (assume_tac o REWRITE_RULE [RC_DEF])) >>
+  fs[] >> fs[] >>
+  metis_tac[RC_DEF,RTC_TRANSITIVE,transitive_def,RTC_SINGLE]
+QED
+
+Theorem rc_diam_to_rtc_diam:
+  ∀tsA tsB wfP.
+    (* ASSUMPTIONS *)
+    (* 1. wfP is preserved by tsA and tsB *)
+    (∀x y.
+      wfP x ∧ tsA x y ⇒ wfP y) ∧
+    (∀x y.
+      wfP x ∧ tsB x y ⇒ wfP y) ∧
+    (* 2. tsA and tsB have RC diamond on wfP states *)
+    (∀S1 S2A S2B.
+      wfP S1 ∧
+      tsA S1 S2A ∧
+      tsB S1 S2B ⇒
+      ∃S3.
+        RC tsB S2A S3 ∧
+        RC tsA S2B S3) ⇒
+    (* CONCLUSION *)
+    (* tsA and tsB have RTC diamond on wfP states*)
+    (∀S1 S2A S2B.
+      wfP S1 ∧
+      RTC tsA S1 S2A ∧
+      RTC tsB S1 S2B ⇒
+      ∃S3.
+        RTC tsB S2A S3 ∧
+        RTC tsA S2B S3)
+Proof
+  ntac 4 strip_tac >>
+  qspecl_then [‘tsA’,‘tsB’,‘wfP’] assume_tac rc_diam_to_srtc_diam >>
+  qmatch_asmsub_abbrev_tac ‘A ⇒ B’ >>
+  ‘B’
+    by (‘A’ suffices_by rw[] >> 
+        qunabbrev_tac ‘A’ >> metis_tac[]) >>
+  qpat_x_assum ‘A ⇒ B’ (K ALL_TAC) >>
+  MAP_EVERY qunabbrev_tac [‘A’,‘B’] >>
+  ntac 2 (last_x_assum assume_tac) >>
+  last_x_assum (K ALL_TAC) >>
+  qspecl_then [‘tsB’,‘RTC tsA’,‘wfP’] assume_tac rc_diam_to_srtc_diam >>
+  ‘RC (RTC tsA) = RTC tsA’
+    by (rw[FUN_EQ_THM,RC_DEF] >>
+        ‘∀a b. (a = b ∨ RTC tsA a b) ⇔ (RTC tsA a b)’
+          by (‘∀a b. a = b ⇒ RTC tsA a b’
+                suffices_by metis_tac[] >>
+              metis_tac[RTC_REFL]) >>
+        fs[]) >>
+  pop_assum (fn x => pop_assum (assume_tac o REWRITE_RULE[x])) >>
+  qmatch_asmsub_abbrev_tac ‘A ⇒ B’ >>
+  ‘B’
+    suffices_by (qunabbrev_tac ‘B’ >> rw[] >>
+                 metis_tac[]) >>
+  ‘A’
+    suffices_by fs[] >>
+  qunabbrev_tac ‘A’ >>
+  ntac 2 (pop_assum (K ALL_TAC)) >>
+  rw[]
+  >- metis_tac[]
+  >- (qpat_x_assum ‘wfP x’ mp_tac >>
+      pop_assum mp_tac >>
+      MAP_EVERY qid_spec_tac [‘x’,‘y’] >>
+      Induct_on ‘RTC’ >>
+      metis_tac[])
+  >- metis_tac[]
+QED
+
+val _ = export_theory ();
