projection/proofs/payloadMiscPropsScript.sml
@@ -1,0 +1,362 @@
+open preamble payloadSemanticsTheory payloadLangTheory;
+
+val _ = new_theory "payloadMiscProps";
+
+val EXISTS_REPLICATE = Q.store_thm("EXISTS_REPLICATE",
+  `!f n d. EXISTS f (REPLICATE n d) = (n > 0 /\ f d)`,
+  Induct_on `n` >> rw[EQ_IMP_THM]);
+
+val unpad_pad = Q.store_thm("unpad_pad",
+  `!conf d. unpad(pad conf d) = TAKE conf.payload_size d`,
+  rw[pad_def,unpad_def,SPLITP_APPEND,EXISTS_REPLICATE,SPLITP]
+  >> TRY(first_x_assum(assume_tac o GSYM)
+         >> rw[TAKE_LENGTH_ID] >> NO_TAC)
+  >> imp_res_tac LESS_IMP_LESS_OR_EQ
+  >> rw[TAKE_LENGTH_TOO_LONG]);
+
+val pad_LENGTH = Q.store_thm("pad_LENGTH",
+  `!conf d. LENGTH(pad conf d) = conf.payload_size + 1`,
+  rw[pad_def]);
+
+val unpad_pad_LENGTH = Q.store_thm("unpad_pad_LENGTH",
+  `!conf d. LENGTH(unpad(pad conf d)) <= conf.payload_size`,
+  rw[unpad_pad,LENGTH_TAKE_EQ]);
+
+val final_pad_LENGTH = Q.store_thm("final_pad_LENGTH",
+  `!conf d. final(pad conf d) <=> LENGTH d <= conf.payload_size`,
+  rw[pad_def,final_def])
+
+val final_pad_TAKE = Q.store_thm("final_pad_TAKE",
+  `!conf d. final(pad conf d) ==> TAKE conf.payload_size d = d`,
+  metis_tac[final_pad_LENGTH,TAKE_LENGTH_TOO_LONG])
+                                  
+val intermediate_pad_LENGTH = Q.store_thm("intermediate_pad_LENGTH",
+  `!conf d. intermediate(pad conf d) <=> conf.payload_size < LENGTH d`,
+  rw[pad_def,intermediate_def])
+
+val pad_not_final = Q.store_thm("pad_not_final",
+  `!conf d. ¬final (pad conf d) <=> intermediate(pad conf d)`,
+  rw[final_def,pad_def,intermediate_def]);
+
+val pad_not_intermediate = Q.store_thm("pad_not_intermediate",
+  `!conf d. ¬intermediate (pad conf d) <=> final(pad conf d)`,
+  metis_tac[pad_not_final]);
+
+val endpoints_def = Define `
+   (endpoints NNil = [])
+/\ (endpoints (NEndpoint p1 s e1) = [(p1,s,e1)])
+/\ (endpoints (NPar n1 n2) = endpoints n1 ++ endpoints n2)`
+
+val reduction_par_l = Q.store_thm("reduction_par_l",
+  `∀p q r conf. (reduction conf)^* p q ==> (reduction conf)^* (NPar p r) (NPar q r)`,
+  rpt gen_tac
+  >> MAP_EVERY (W(curry Q.SPEC_TAC)) [`q`,`p`]
+  >> ho_match_mp_tac RTC_INDUCT
+  >> rpt strip_tac
+  >- simp[RTC_REFL]
+  >> match_mp_tac (RTC_RULES |> SPEC_ALL |> CONJUNCT2)
+  >> metis_tac[reduction_def,trans_par_l]);
+
+val reduction_par_r = Q.store_thm("reduction_par_r",
+  `∀p q r conf. (reduction conf)^* p q ==> (reduction conf)^* (NPar r p) (NPar r q)`,
+  rpt gen_tac
+  >> MAP_EVERY (W(curry Q.SPEC_TAC)) [`q`,`p`]
+  >> ho_match_mp_tac RTC_INDUCT
+  >> rpt strip_tac
+  >- simp[RTC_REFL]
+  >> match_mp_tac (RTC_RULES |> SPEC_ALL |> CONJUNCT2)
+  >> metis_tac[reduction_def,trans_par_r]);
+
+val trans_nil_false = Q.store_thm("trans_nil_false",
+  `∀conf alpha n. trans conf NNil alpha n = F`,
+  rpt strip_tac
+  >> PURE_ONCE_REWRITE_TAC[trans_cases]
+  >> fs[]);
+
+val reduction_par_l = Q.store_thm("reduction_par_l",
+  `∀p q r conf. (reduction conf)^* p q ==> (reduction conf)^* (NPar p r) (NPar q r)`,
+  rpt gen_tac
+  >> MAP_EVERY (W(curry Q.SPEC_TAC)) [`q`,`p`]
+  >> ho_match_mp_tac RTC_INDUCT
+  >> rpt strip_tac
+  >- simp[RTC_REFL]
+  >> match_mp_tac (RTC_RULES |> SPEC_ALL |> CONJUNCT2)
+  >> metis_tac[reduction_def,trans_par_l]);
+
+val reduction_par_r = Q.store_thm("reduction_par_r",
+  `∀p q r conf. (reduction conf)^* p q ==> (reduction conf)^* (NPar r p) (NPar r q)`,
+  rpt gen_tac
+  >> MAP_EVERY (W(curry Q.SPEC_TAC)) [`q`,`p`]
+  >> ho_match_mp_tac RTC_INDUCT
+  >> rpt strip_tac
+  >- simp[RTC_REFL]
+  >> match_mp_tac (RTC_RULES |> SPEC_ALL |> CONJUNCT2)
+  >> metis_tac[reduction_def,trans_par_r]);
+
+val trans_nil_false = Q.store_thm("trans_nil_false",
+  `∀conf alpha n. trans conf NNil alpha n = F`,
+  rpt strip_tac
+  >> PURE_ONCE_REWRITE_TAC[trans_cases]
+  >> fs[]);
+
+val reduction_nil = Q.store_thm("reduction_nil",
+  `∀conf n. (reduction conf)^* NNil n ==> n = NNil`,
+  rpt strip_tac
+  >> qpat_abbrev_tac `a1 = NNil`
+  >> pop_assum (assume_tac o REWRITE_RULE[markerTheory.Abbrev_def])
+  >> simp[]
+  >> rpt(last_x_assum mp_tac)
+  >> PURE_ONCE_REWRITE_TAC [AND_IMP_INTRO]
+  >> MAP_EVERY (W(curry Q.SPEC_TAC)) [`n`,`a1`]
+  >> ho_match_mp_tac RTC_lifts_invariants
+  >> simp[payloadSemanticsTheory.reduction_def,trans_nil_false]);
+
+val list_trans_def = Define `
+    (list_trans conf p [] q = (p = q))
+ /\ (list_trans conf p (alpha::l) q = ?p'. trans conf p alpha p' /\ list_trans conf p' l q)`
+
+val list_trans_append = Q.store_thm("list_trans_append",
+  `!l1 n1 l2 n2 conf. list_trans conf n1 (l1 ++ l2) n2 =
+  ?n3. list_trans conf n1 l1 n3 /\ list_trans conf n3 l2 n2`,
+  Induct_on `l1` >> rpt strip_tac >> fs[list_trans_def]
+  >> rw[EQ_IMP_THM] >> fs[] >> metis_tac[]);
+
+val list_trans_par_l = Q.store_thm("list_trans_par_l",
+  `∀conf p alpha q r. list_trans conf p alpha q ==> list_trans conf (NPar p r) alpha (NPar q r)`,
+  Induct_on `alpha`
+  >- simp[list_trans_def]
+  >> rpt strip_tac
+  >> fs[list_trans_def] >> metis_tac[payloadSemanticsTheory.trans_par_l]);
+
+val list_trans_par_r = Q.store_thm("list_trans_par_r",
+  `∀conf p alpha q r. list_trans conf p alpha q ==> list_trans conf (NPar r p) alpha (NPar r q)`,
+  Induct_on `alpha`
+  >- simp[list_trans_def]
+  >> rpt strip_tac
+  >> fs[list_trans_def] >> metis_tac[payloadSemanticsTheory.trans_par_r]);
+
+val endpoint_names_trans = Q.store_thm("endpoint_names_trans",
+  `!conf n1 alpha n2. trans conf n1 alpha n2 ==> MAP FST (endpoints n2) = MAP FST(endpoints n1)`,
+  ho_match_mp_tac trans_strongind >> rpt strip_tac >> fs[endpoints_def]);
+
+val endpoint_names_list_trans = Q.store_thm("endpoint_names_list_trans",
+  `!conf n1 alpha n2. list_trans conf n1 alpha n2 ==> MAP FST (endpoints n2) = MAP FST(endpoints n1)`,
+  Induct_on `alpha` >> rw[list_trans_def] >>
+  metis_tac[endpoint_names_trans]);
+
+val sender_is_endpoint = Q.store_thm("sender_is_endpoint",
+ `∀p1 p2 q1 d q2 conf.
+  trans conf p1 (LSend q1 d q2) p2 ==> MEM q1 (MAP FST (endpoints p1))`,
+  rpt strip_tac
+  >> qmatch_asmsub_abbrev_tac `trans _ _ alpha _`
+  >> pop_assum (mp_tac o REWRITE_RULE[markerTheory.Abbrev_def])
+  >> MAP_EVERY (W(curry Q.SPEC_TAC)) [`q1`,`d`,`q2`]
+  >> pop_assum mp_tac
+  >> MAP_EVERY (W(curry Q.SPEC_TAC)) [`p2`,`alpha`,`p1`,`conf`]
+  >> ho_match_mp_tac trans_strongind
+  >> rpt strip_tac >> fs[] >> rveq
+  >> fs[endpoints_def]);
+
+val receiver_is_endpoint = Q.store_thm("receiver_is_endpoint",
+ `∀p1 p2 q1 d q2 conf.
+  trans conf p1 (LReceive q1 d q2) p2 ==> MEM q2 (MAP FST (endpoints p1))`,
+  rpt strip_tac
+  >> qmatch_asmsub_abbrev_tac `trans _ _ alpha _`
+  >> pop_assum (mp_tac o REWRITE_RULE[markerTheory.Abbrev_def])
+  >> MAP_EVERY (W(curry Q.SPEC_TAC)) [`q1`,`d`,`q2`]
+  >> pop_assum mp_tac
+  >> MAP_EVERY (W(curry Q.SPEC_TAC)) [`p2`,`alpha`,`p1`,`conf`]
+  >> ho_match_mp_tac trans_strongind
+  >> rpt strip_tac >> fs[] >> rveq
+  >> fs[endpoints_def]);
+
+val add_queue_def = Define `
+  (add_queue p1 qe p2 payloadLang$NNil = NNil)
+  ∧ (add_queue p1 qe p2 (NEndpoint p s e) =
+      if p1 = p then NEndpoint p (s with queue := SNOC (p2,qe) s.queue) e
+      else NEndpoint p s e
+     )
+  ∧ (add_queue p1 qe p2 (NPar n1 n2) = NPar (add_queue p1 qe p2 n1) (add_queue p1 qe p2 n2))
+`
+
+Theorem trans_same_sender_determ:
+  trans conf p1 (LSend q2 d1 q1) p2
+  /\ trans conf p1 (LSend q2 d2 q3) p3
+  /\ ALL_DISTINCT(MAP FST(endpoints p1))
+  ==> q1 = q3 /\ d1 = d2 /\ p2 = p3
+Proof
+  qmatch_goalsub_abbrev_tac `trans _ _ alpha`
+  >> rpt(disch_then strip_assume_tac)
+  >> pop_assum mp_tac
+  >> qhdtm_x_assum `Abbrev` (mp_tac o REWRITE_RULE[markerTheory.Abbrev_def])
+  >> rpt(pop_assum mp_tac)
+  >> MAP_EVERY qid_spec_tac [`q2`,`d2`,`q1`,`d1`,`p3`,`q3`,`p2`,`alpha`,`p1`,`conf`]
+  >> Ho_Rewrite.PURE_REWRITE_TAC[GSYM PULL_FORALL]
+  >> ho_match_mp_tac trans_strongind
+  >> rpt conj_tac >> rpt(gen_tac ORELSE disch_then strip_assume_tac)
+  >> fs[] >> rveq
+  >> qhdtm_x_assum `trans` (assume_tac o SIMP_RULE std_ss [Once trans_cases])
+  >> fs[] >> rveq >> fs[] >> rveq >> fs[endpoints_def,ALL_DISTINCT_APPEND]
+  >> metis_tac[sender_is_endpoint]
+QED
+
+Theorem trans_same_receiver_determ:
+  trans conf p1 (LReceive s d r) p2
+  /\ trans conf p1 (LReceive s d r) p3
+  /\ ALL_DISTINCT(MAP FST(endpoints p1))
+  ==> p2 = p3
+Proof
+  qmatch_goalsub_abbrev_tac `trans _ _ alpha`
+  >> rpt(disch_then strip_assume_tac)
+  >> pop_assum mp_tac
+  >> qhdtm_x_assum `Abbrev` (mp_tac o REWRITE_RULE[markerTheory.Abbrev_def])
+  >> rpt(pop_assum mp_tac)
+  >> MAP_EVERY qid_spec_tac [`p3`,`s`,`d`,`r`,`p2`,`alpha`,`p1`,`conf`]
+  >> Ho_Rewrite.PURE_REWRITE_TAC[GSYM PULL_FORALL]
+  >> ho_match_mp_tac trans_strongind
+  >> rpt conj_tac >> rpt(gen_tac ORELSE disch_then strip_assume_tac)
+  >> fs[] >> rveq
+  >> qhdtm_x_assum `trans` (assume_tac o SIMP_RULE std_ss [Once trans_cases])
+  >> fs[] >> rveq >> fs[] >> rveq >> fs[endpoints_def,ALL_DISTINCT_APPEND]
+  >> metis_tac[receiver_is_endpoint]
+QED
+
+Theorem trans_no_selfloop:
+  !conf p1 alpha p2.
+  trans conf p1 alpha p2 /\ conf.payload_size > 0
+  ==> p1 <> p2
+Proof
+  PURE_REWRITE_TAC[GSYM AND_IMP_INTRO] >>
+  ho_match_mp_tac trans_ind >> rw[] >> fs[endpointLangTheory.state_component_equality] >>
+  TRY(disj2_tac) >> spose_not_then strip_assume_tac >>
+  qmatch_asmsub_abbrev_tac `a1 = a2` >>
+  `endpoint_size a1 = endpoint_size a2` by simp[] >>
+  pop_assum mp_tac >> unabbrev_all_tac >> rpt(pop_assum kall_tac) >>
+  simp[endpoint_size_def]
+QED
+
+Theorem trans_different_sender:
+  trans conf p1 (LSend s1 d1 r1) p2
+  /\ trans conf p1 (LSend s2 d2 r2) p3
+  /\ conf.payload_size > 0
+  /\ s1 <> s2
+  ==> p2 <> p3
+Proof
+  qmatch_goalsub_abbrev_tac `trans _ _ alpha`
+  >> rpt(disch_then strip_assume_tac)
+  >> pop_assum mp_tac
+  >> qhdtm_x_assum `Abbrev` (mp_tac o REWRITE_RULE[markerTheory.Abbrev_def])
+  >> rpt(pop_assum mp_tac)
+  >> MAP_EVERY qid_spec_tac [`r2`,`r1`,`d2`,`s2`,`d1`,`p3`,`s1`,`p2`,`alpha`,`p1`,`conf`]
+  >> Ho_Rewrite.PURE_REWRITE_TAC[GSYM PULL_FORALL]
+  >> ho_match_mp_tac trans_strongind
+  >> rpt conj_tac >> rpt(gen_tac ORELSE disch_then strip_assume_tac)
+  >> fs[] >> rveq
+  >> qhdtm_x_assum `trans` (assume_tac o SIMP_RULE std_ss [Once trans_cases])
+  >> fs[] >> rveq >> fs[] >> rveq >> fs[endpoints_def,ALL_DISTINCT_APPEND]
+  >> metis_tac[sender_is_endpoint,trans_no_selfloop]
+QED
+
+(* TODO: remove? strictly weaker than trans_distinct_residual *)
+Theorem trans_send_receive_distinct:
+  trans conf p1 (LSend s1 d1 r1) p2
+  /\ trans conf p1 (LReceive s2 d2 r2) p3
+  /\ conf.payload_size > 0 (* not strictly needed *)
+  ==> p2 <> p3
+Proof
+  qmatch_goalsub_abbrev_tac `trans _ _ alpha`
+  >> rpt(disch_then strip_assume_tac)
+  >> pop_assum mp_tac
+  >> qhdtm_x_assum `Abbrev` (mp_tac o REWRITE_RULE[markerTheory.Abbrev_def])
+  >> rpt(pop_assum mp_tac)
+  >> MAP_EVERY qid_spec_tac [`r2`,`r1`,`d2`,`s2`,`d1`,`p3`,`s1`,`p2`,`alpha`,`p1`,`conf`]
+  >> Ho_Rewrite.PURE_REWRITE_TAC[GSYM PULL_FORALL]
+  >> ho_match_mp_tac trans_strongind
+  >> rpt conj_tac >> rpt(gen_tac ORELSE disch_then strip_assume_tac)
+  >> fs[] >> rveq
+  >> qhdtm_x_assum `trans` (assume_tac o SIMP_RULE std_ss [Once trans_cases])
+  >> fs[] >> rveq >> fs[] >> rveq >> fs[endpoints_def,ALL_DISTINCT_APPEND]
+  >> fs[endpointLangTheory.state_component_equality]
+  >> metis_tac[sender_is_endpoint,trans_no_selfloop]
+QED
+
+Theorem trans_distinct_residual:
+  !conf p1 alpha p2 beta p3.
+  trans conf p1 alpha p2
+  /\ trans conf p1 beta p3
+  /\ alpha <> beta
+  /\ conf.payload_size > 0
+  ==> p2 <> p3
+Proof
+  Ho_Rewrite.PURE_REWRITE_TAC[GSYM PULL_FORALL,GSYM AND_IMP_INTRO] >>
+  ho_match_mp_tac trans_strongind >> rpt strip_tac >>
+  fs[] >> rveq
+  >- (* Send-last-payload *)
+     (qhdtm_x_assum `trans` (assume_tac o SIMP_RULE std_ss [Once trans_cases]) >>
+      fs[] >> rveq >> fs[] >> rveq >> fs[endpointLangTheory.state_component_equality])
+  >- (* Send-intermediate-payload *)
+     (qhdtm_x_assum `trans` (assume_tac o SIMP_RULE std_ss [Once trans_cases]) >>
+      fs[] >> rveq >> fs[] >> rveq >> fs[endpointLangTheory.state_component_equality])
+  >- (* Enqueue *)
+     (qhdtm_x_assum `trans` (assume_tac o SIMP_RULE std_ss [Once trans_cases]) >>
+      fs[] >> rveq >> fs[] >> rveq >> fs[endpointLangTheory.state_component_equality] >>
+      qmatch_asmsub_abbrev_tac `a1:endpoint = a2` >>
+      `endpoint_size a1 = endpoint_size a2` by simp[] >>
+      unabbrev_all_tac >> pop_assum mp_tac >> rpt(pop_assum kall_tac) >>
+      simp[endpoint_size_def])
+  >- (* Com-L *)
+     (qhdtm_x_assum `trans` (assume_tac o SIMP_RULE std_ss [Once trans_cases]) >>
+      fs[] >> rveq >> fs[] >> rveq >> fs[] >>
+      Cases_on `beta` >> fs[] >> metis_tac[trans_no_selfloop])
+  >- (* Com-R *)
+     (qhdtm_x_assum `trans` (assume_tac o SIMP_RULE std_ss [Once trans_cases]) >>
+      fs[] >> rveq >> fs[] >> rveq >> fs[] >>
+      Cases_on `beta` >> fs[] >> metis_tac[trans_no_selfloop])
+  >- (* Dequeue-last-payload *)
+     (qhdtm_x_assum `trans` (assume_tac o SIMP_RULE std_ss [Once trans_cases]) >>
+      fs[] >> rveq >> fs[] >> rveq >> fs[endpointLangTheory.state_component_equality] >>
+      qmatch_asmsub_abbrev_tac `a1:endpoint = a2` >>
+      `endpoint_size a1 = endpoint_size a2` by simp[] >>
+      unabbrev_all_tac >> pop_assum mp_tac >> rpt(pop_assum kall_tac) >>
+      simp[endpoint_size_def])
+  >- (* Dequeue-intermediate-payload *)
+     (qhdtm_x_assum `trans` (assume_tac o SIMP_RULE std_ss [Once trans_cases]) >>
+      fs[] >> rveq >> fs[] >> rveq >> fs[endpointLangTheory.state_component_equality] >>
+      qmatch_asmsub_abbrev_tac `a1:endpoint = a2` >>
+      `endpoint_size a1 = endpoint_size a2` by simp[] >>
+      unabbrev_all_tac >> pop_assum mp_tac >> rpt(pop_assum kall_tac) >>
+      simp[endpoint_size_def])
+  >- (* If-L *)
+     (qhdtm_x_assum `trans` (assume_tac o SIMP_RULE std_ss [Once trans_cases]) >>
+      fs[] >> rveq >> fs[] >> rveq >> fs[endpointLangTheory.state_component_equality])
+  >- (* If-R *)
+     (qhdtm_x_assum `trans` (assume_tac o SIMP_RULE std_ss [Once trans_cases]) >>
+      fs[] >> rveq >> fs[] >> rveq >> fs[endpointLangTheory.state_component_equality])
+  >- (* Let *)
+     (qhdtm_x_assum `trans` (assume_tac o SIMP_RULE std_ss [Once trans_cases]) >>
+      fs[] >> rveq >> fs[] >> rveq >> fs[endpointLangTheory.state_component_equality])
+  >- (* Par-L *)
+     (qhdtm_x_assum `trans` (assume_tac o SIMP_RULE std_ss [Once trans_cases]) >>
+      fs[] >> rveq >> fs[] >> rveq >> fs[] >> metis_tac[trans_no_selfloop])
+  >- (* Par-R *)
+     (qhdtm_x_assum `trans` (assume_tac o SIMP_RULE std_ss [Once trans_cases]) >>
+      fs[] >> rveq >> fs[] >> rveq >> fs[] >> metis_tac[trans_no_selfloop])
+QED
+
+Theorem intermediate_final_IMP:
+  !d. intermediate d /\ final d ==> F
+Proof
+  Cases >> rpt strip_tac >> fs[intermediate_def,final_def] >> rveq >> fs[]
+QED
+
+Theorem qcong_list_trans_pres:
+  !conf p l q p'. list_trans conf p l q /\ qcong p p'
+  ==> ?q'. list_trans conf p' l q' /\ qcong q q'
+Proof
+  Induct_on `l` >>
+  rw[list_trans_def] >> simp[] >>
+  dxrule_all_then strip_assume_tac qcong_trans_pres >>
+  metis_tac[]
+QED
+
+val _ = export_theory ();
